Update Fin_inv.v

src/Fin_inv.v
@@ -6,6 +6,159 @@ Notation "'Sigma' x .. y , p" :=
      format "'[' 'Sigma'  '/  ' x  ..  y ,  '/  ' p ']'")
   : type_scope.
 
+Theorem fin_inv : ∀ (n : nat) (f : Fin.t n), 
+  match n as np return n = np -> Fin.t np -> Type 
+  with 
+  | 0 => fun Ha _  => False
+  | S n'  => fun Ha ft => ((ft = @Fin.F1 n') + Sigma (u : Fin.t n'), ft = Fin.FS u)%type
+  end eq_refl f.
+Proof.
+  destruct n as [|n].
+  +
+    intro Ha.
+    refine match Ha with end.
+  +
+    intros f.
+    refine 
+      match f with 
+      | Fin.F1 => _
+      | Fin.FS t => _ 
+      end; [left | right].
+    ++
+      exact eq_refl.
+    ++
+      exists t; exact eq_refl.
+Defined.
+
+
+Theorem fin_inv_destruct : ∀ (n : nat) (f : Fin.t n), 
+  match n return Fin.t n -> Type 
+  with 
+  | 0 => fun _  => IDProp
+  | S n'  => fun ft => ((ft = @Fin.F1 n') + Sigma (u : Fin.t n'), ft = Fin.FS u)%type
+  end f.
+Proof.
+  intros *.
+  destruct f as [|f'];
+  [left; exact eq_refl | right].
+  exists f. exact eq_refl.
+Defined.
+
+
+Theorem fin_inv_convoy : ∀ (n : nat) (f : Fin.t n), 
+  match n return Fin.t n -> Type 
+  with 
+  | 0 => fun _  => IDProp
+  | S n'  => fun ft => ((ft = @Fin.F1 n') + Sigma (u : Fin.t n'), ft = Fin.FS u)%type
+  end f.
+Proof.
+  intros *.
+  refine
+    (match f as f' in Fin.t n' return 
+      (match n' return Fin.t n' -> Type 
+      with 
+      | 0 => fun _  => IDProp
+      | S n'  => fun ft => ((ft = @Fin.F1 n') + 
+        Sigma (u : Fin.t n'), ft = Fin.FS u)%type
+      end f')
+    with 
+    | Fin.F1 => inl eq_refl
+    | Fin.FS f' => inr (exist _ f' eq_refl)
+    end). 
+Defined.
+
+
+Definition Fin_t_0_inv i : ∀ (P : t 0 → Type), P i :=
+  match i with end.
+
+
+(* This is the most powerful induction scheme*)
+Definition Fin_t_S_inv n i :
+  ∀ (P : t (S n) → Type), P F1 → (∀i, P (FS i)) → P i.
+Proof.
+  refine 
+  (match i as i' in Fin.t n' return 
+    (match n' as n'' return (Fin.t n'' → Type) with
+    | 0 => fun _ => IDProp
+    | S n'' => fun (ea : Fin.t (S n'')) =>
+       ∀ (P : t (S n'') → Type), P F1 → 
+       (∀ (eb : Fin.t n''), P (FS eb)) → P ea 
+    end i')
+  with
+  | F1 => _ 
+  | FS j => _ 
+  end). 
+  +
+    intros * ha hb.
+    exact ha.
+  +
+    intros * ha hb.
+    exact (hb j).
+Defined.
+
+(* this can proven from the top one Fin_t_S_inv *)
+Lemma Fin_t_S_inv_convoy : ∀ (n : nat) (P : t (S n) → Type),
+   P F1 → (∀ (i : Fin.t n), P (FS i)) →  ∀ (i : Fin.t (S n)), P i.
+Proof.
+  intros * ha hb i.
+  (* 
+  eapply Fin_t_S_inv.
+  exact ha. eapply hb.
+  *)
+  refine
+  (match i as i' in Fin.t n'
+    return 
+    ∀ (pfa : S n = n'),
+    (match n' as n'' return n' = n'' -> Fin.t n'' -> Type 
+    with 
+    | 0 => fun _ _ => IDProp 
+    | S n'' => fun (pfb : n' = S n'') (f : Fin.t (S n'')) => 
+      P (eq_rect (S n'') Fin.t f _ (eq_sym (eq_trans pfa pfb))) 
+    end eq_refl i')
+  with 
+  | Fin.F1 => fun pfa => _ 
+  | Fin.FS f' => fun pfa => _ 
+  end eq_refl); cbn;
+  inversion pfa as [pfaa]; subst;
+  assert (pfa = eq_refl) by apply Eqdep_dec.UIP_refl_nat;
+  subst; cbn; [exact ha | exact (hb f')].
+Defined.
+
+(* This can be proven from Fin_t_S_inv_convoy *)
+Lemma Fin_t_S_inv_gen_convoy : ∀ (P : ∀ (n : nat), t (S n) → Type),
+   (∀ (n : nat), P n F1) → 
+   (∀ (n : nat) (i : Fin.t n), P n (FS i)) →  
+   ∀ (n : nat) (i : Fin.t (S n)), P n i.
+Proof.
+  intros * ha hb *.
+  (* 
+  eapply Fin_t_S_inv_convoy.
+  apply ha. apply hb.
+  *)
+  refine
+  (match i as i' in Fin.t n' return 
+    (match n' return Fin.t n' -> Type 
+    with 
+    | 0 => fun _ => IDProp
+    | S n'' => fun (e : Fin.t (S n'')) =>
+      P _ e 
+    end i')
+  with 
+  | @Fin.F1 nw => ha nw 
+  | @Fin.FS nw f' => hb nw f'
+  end). 
+Defined.
+
+(* Below code will not go through *)
+
+Require Import Fin Utf8.
+
+Notation "'Sigma' x .. y , p" :=
+  (sig (fun x => .. (sig (fun y => p)) ..))
+    (at level 200, x binder, right associativity,
+     format "'[' 'Sigma'  '/  ' x  ..  y ,  '/  ' p ']'")
+  : type_scope.
+
 
 Theorem fin_inv : ∀ (n : nat) (f : Fin.t n), 
   match n as np return n = np -> Fin.t np -> Type 
